Automata/RegEx/NFA.lean
@@ -1,0 +1,84 @@
+import Automata.RegEx.Basic
+import Automata.NFA
+
+namespace RegEx
+
+/-- Regular expresion compiler -/
+def compile : RegEx α → NFA α
+  | empty => NFA.false
+  | nil => NFA.eps
+  | lit s => NFA.lit s
+  | alt a b => compile a ||| compile b
+  | cat a b => compile a ++ compile b
+  | star a => (compile a).star
+
+theorem soundness (h : Language a xs) : (compile a).accept xs := by
+  induction h with
+  | nil => exact NFA.eps_sound rfl
+  | lit h => exact NFA.lit_sound _ h
+  | altL _ ih => exact NFA.alt_sound_left ih
+  | altR _ ih => exact NFA.alt_sound_right  ih
+  | cat _ _ ih₁ ih₂ => exact NFA.cat_sound ih₁ ih₂
+  | starNil => exact NFA.star_sound_nil _
+  | starCat _ _ ih₁ ih₂ => exact NFA.star_sound_append _ ih₁ ih₂
+
+theorem completeness (h : (compile a).accept xs) : Language a xs :=
+  match a, xs with
+  | nil, zs => by
+    simp only [compile] at h
+    rw [NFA.eps_correct] at h
+    split at h
+    next => exact Language.nil
+    next => contradiction
+  | lit s, zs => by
+    simp only [compile] at h
+    rw [NFA.lit_correct] at h
+    split at h
+    next x => exact Language.lit h
+    next => contradiction
+  | alt a b, _ => by
+    simp only [compile] at h
+    cases NFA.alt_exact h with
+    | inl hl =>
+      apply Language.altL
+      exact completeness hl
+    | inr hr =>
+      apply Language.altR
+      exact completeness hr
+  | cat a b, zs => by
+    simp only [compile] at h
+    match NFA.cat_exact h with
+    | ⟨xs, ys, heq, ha, hb⟩ =>
+      rw [heq]
+      apply Language.cat
+      · exact completeness ha
+      · exact completeness hb
+  | star a, zs => by
+    simp only [compile] at h
+    if hz : zs = [] then
+      rw [hz]
+      apply Language.starNil
+    else
+      match NFA.star_exact (compile a) h hz with
+      | ⟨xs, ys, hxs, heq, hx, hy⟩ =>
+        have : 1 ≤ xs.length := by
+          cases xs with
+          | nil => contradiction
+          | cons => rw [List.length_cons]; omega
+        rw [heq]
+        apply Language.starCat
+        · exact completeness hx
+        · have : 1 + sizeOf a + ys.length < 1 + sizeOf a + zs.length := by
+            rw [heq, List.length_append]; omega
+          exact completeness hy
+  | empty, _ => by
+    simp only [compile] at h
+    rw [NFA.false_correct] at h
+    contradiction
+termination_by sizeOf a + List.length xs
+
+theorem exact (xs : List α) : (compile a).accept xs ↔ Language a xs := ⟨completeness, soundness⟩
+
+instance (xs : List α) : Decidable (Language a xs) := decidable_of_decidable_of_iff (exact xs)
+
+end RegEx
